theories/aneris_lang/adequacy.v
@@ -8,8 +8,9 @@ Set Default Proof Using "Type".
 
 Import Network.
 
-Theorem adequacy `{anerisPreG Σ} IPs A s e ip σ φ (ports : gset port) :
-  (∀ `{anerisG Σ}, ⊢ |={⊤}=> ∃ (f : socket_address → socket_interp Σ),
+Theorem adequacy `{anerisPreG Σ Mdl} IPs A s e ip σ φ (ports : gset port)
+  (st0 : Mdl) :
+  (∀ `{anerisG Mdl Σ}, ⊢ |={⊤}=> ∃ (f : socket_address → socket_interp Σ),
      fixed A -∗ ([∗ set] a ∈ A, a ⤇ (f a)) -∗
      ([∗ set] i ∈ IPs, free_ip i) -∗ is_node ip -∗
      WP (mkExpr ip e) @ s; ⊤ {{v, ⌜φ v⌝ }}) →
@@ -24,7 +25,8 @@ Theorem adequacy `{anerisPreG Σ} IPs A s e ip σ φ (ports : gset port) :
   adequate s (mkExpr ip e) σ (λ v _, φ v).
 Proof.
   intros Hwp Hps Hipdom Hpiiu Hip Hfixdom Hste Hsce Hmse.
-  eapply (wp_adequacy _ aneris_AS _ _ _ _ ());
+  set (δ := @AnerisAuxState Mdl (history_init ip ports) st0).
+  eapply (wp_adequacy _ (@aneris_AS Mdl) _ _ _ _  (δ  : aux_state aneris_AS));
     first apply aneris_AS_valid_state_evolution_finitary.
   iIntros (?) "/=".
   iMod node_gnames_auth_init as (γmp) "Hmp".
@@ -33,6 +35,7 @@ Proof.
   iMod (free_ips_init IPs) as (γips) "[HIPsCtx HIPs]".
   iMod free_ports_auth_init as (γpiu) "HPiu".
   iMod (gen_heap_light_init (history_init ip ports)) as (γms) "Hms".
+  iMod (model_init st0) as (γm) "Hmdl".
   set (dg :=
          {|
            aneris_node_gnames_name := γmp;
@@ -40,7 +43,8 @@ Proof.
            aneris_fixed_name := γsif;
            aneris_freeips_name := γips;
            aneris_freeports_name := γpiu;
-           aneris_messages_name := γms
+           aneris_messages_name := γms;
+           anerisG_model_name := γm;
          |}).
   iMod (Hwp dg) as (f) "Hwp".
   iMod (saved_si_update A with "[$Hsi $Hsi']") as (M HMfs) "[HM #Hsa]".
@@ -58,19 +62,21 @@ Proof.
   iAssert (is_node ip) as "Hn".
   { iExists _. eauto. }
   iModIntro.
-  iExists (λ σ _ _, aneris_state_interp σ), (λ _, True)%I.
+  iExists  (λ σ δ _, aneris_state_interp σ _), (λ _, True)%I.
   iSplitR; last first.
   iSplitR "Hwp HIPs"; last first.
   { iApply ("Hwp" with "Hsif Hsa' HIPs Hn"). }
-  iApply (@aneris_state_interp_init _ dg with
-              "[Hmp] [] [Hh] [Hs] [Hms] [] [HM] [] [HIPsCtx]  [HPiu]"); eauto.
-  iApply config_wp_correct.
+  iPoseProof (@aneris_state_interp_init _ _ dg IPs _ _ _ _ _ ports
+                with "[Hmp] [] [Hh] [Hs] [Hms] [] [HM] [] [HIPsCtx] [HPiu] ")
+    as "Hsi"; eauto.
+    iApply config_wp_correct.
 Qed.
 
 Definition safe e σ := @adequate aneris_lang NotStuck e σ (λ _ _, True).
 
-Theorem adequacy_safe `{anerisPreG Σ} IPs A e ip σ (ports : gset port):
-  (∀ `{anerisG Σ}, ⊢ |={⊤}=> ∃ (f : socket_address → socket_interp Σ),
+Theorem adequacy_safe `{anerisPreG Σ Mdl} IPs A e ip σ (ports : gset port)
+        (st0 : Mdl):
+  (∀ `{anerisG Mdl Σ}, ⊢ |={⊤}=> ∃ (f : socket_address → socket_interp Σ),
      fixed A -∗ ([∗ set] a ∈ A, a ⤇ (f a)) -∗
      ([∗ set] i ∈ IPs, free_ip i) -∗ is_node ip -∗
      WP (mkExpr ip e) {{v, True }}) →
@@ -83,10 +89,11 @@ Theorem adequacy_safe `{anerisPreG Σ} IPs A e ip σ (ports : gset port):
   state_sockets σ = {[ip:=∅]} →
   state_ms σ = ∅ →
   safe (mkExpr ip e) σ.
-Proof. apply adequacy. Qed.
+Proof. by apply adequacy. Qed.
 
-Theorem adequacy_hoare `{anerisPreG Σ} IPs A e σ φ ip (ports : gset port):
-  (∀ `{anerisG Σ}, ⊢ ∃ (f : socket_address → socket_interp Σ),
+Theorem adequacy_hoare `{anerisPreG Σ Mdl} IPs A e σ φ ip (ports : gset port)
+  (st0 : Mdl) :
+  (∀ `{anerisG Mdl Σ}, ⊢ ∃ (f : socket_address → socket_interp Σ),
           {{{ fixed A
             ∗ ([∗ set] a ∈ A, a ⤇ (f a))
             ∗ ([∗ set] ip ∈ IPs, free_ip ip) ∗ is_node ip }}}
@@ -103,7 +110,7 @@ Theorem adequacy_hoare `{anerisPreG Σ} IPs A e σ φ ip (ports : gset port):
   adequate NotStuck (mkExpr ip e) σ (λ v _, φ v).
 Proof.
   intros Hwp ????????.
-  eapply adequacy; [|done..].
+  eapply (adequacy _ _ _ _ _ _ _ _ st0); try eauto.
   intros ?. iModIntro.
   iDestruct Hwp as (f) "#Hwp".
   iExists f. iIntros "????".
