theories/aneris_lang/program_logic/aneris_adequacy.v
@@ -8,8 +8,8 @@ Definition aneris_adequate (e : base_lang.expr) (ip : ip_address) (σ : state)
            (φ : base_lang.val → Prop) :=
   adequate NotStuck (mkExpr ip e) σ (λ v _, ∃ w, v = mkVal ip w ∧ φ w).
 
-Theorem adequacy `{anerisPreG Σ} IPs A e ip σ φ (ports : gset port) :
-  (∀ `{anerisG Σ}, ⊢ |={⊤}=> ∃ (f : socket_address → socket_interp Σ),
+Theorem adequacy `{anerisPreG Σ Mdl} IPs A e ip σ φ (ports : gset port) :
+  (∀ `{anerisG Mdl Σ}, ⊢ |={⊤}=> ∃ (f : socket_address → socket_interp Σ),
      fixed A -∗ ([∗ set] a ∈ A, a ⤇ (f a)) -∗
      ([∗ set] i ∈ IPs, free_ip i) -∗
      WP e @[ip] ⊤ {{ v, ⌜φ v⌝ }}) →
@@ -34,8 +34,8 @@ Proof.
   eauto.
 Qed.
 
-Theorem adequacy_hoare `{anerisPreG Σ} IPs A e σ φ ip (ports : gset port) :
-  (∀ `{anerisG Σ}, ⊢ ∃ (f : socket_address → socket_interp Σ),
+Theorem adequacy_hoare `{anerisPreG Σ Mdl} IPs A e σ φ ip (ports : gset port) :
+  (∀ `{anerisG Mdl Σ}, ⊢ ∃ (f : socket_address → socket_interp Σ),
       {{{ fixed A ∗ ([∗ set] a ∈ A, a ⤇ (f a)) ∗ ([∗ set] ip ∈ IPs, free_ip ip) }}}
           e @[ip]
       {{{ v, RET v; ⌜φ v⌝ }}}) →
